src/example/treiber/ClientSpecHOCAP.v
@@ -1,0 +1,313 @@
+From sflib Require Import sflib.
+From Paco Require Import paco.
+Require Import Coq.Classes.RelationClasses Lia Program.
+From Fairness Require Import pind Axioms ITreeLib Red TRed IRed2 WFLibLarge.
+From Fairness Require Import FairBeh Mod Concurrency Linking.
+From Fairness Require Import PCM IProp IPM IPropAux.
+From Fairness Require Import IndexedInvariants OpticsInterp SimWeakest SimWeakestAdequacy.
+From Fairness Require Import TemporalLogic SCMemSpec ghost_map ghost_excl LifetimeRA AuthExclsRA.
+From Fairness.treiber Require Import ClientCode SpecHOCAP.
+
+Section SPEC.
+
+  Notation src_state := (Mod.state TreiberClientSpec.module).
+  Notation src_ident := (Mod.ident TreiberClientSpec.module).
+  Notation tgt_state := (Mod.state TreiberClient.module).
+  Notation tgt_ident := (Mod.ident TreiberClient.module).
+
+  Local Instance STT : StateTypes := Build_StateTypes src_state tgt_state src_ident tgt_ident.
+  Context `{sub : @SRA.subG Γ Σ}.
+  Context {TLRASs : TLRAs_small STT Γ}.
+  Context {TLRAS : TLRAs STT Γ Σ}.
+
+  Context {HasMemRA: @GRA.inG memRA Γ}.
+  Context {HasLifetime : @GRA.inG Lifetime.t Γ}.
+
+  Context {HasAuthExclsRAlist : @GRA.inG (AuthExcls.t (list SCMem.val)) Γ}.
+  Context {HasGhostMap : @GRA.inG (ghost_mapURA nat maybe_null_ptr) Γ}.
+  Context {HasGhostExcl : @GRA.inG (ghost_exclURA unit) Γ}.
+
+  Ltac red_tl_all := red_tl; red_tl_memra; red_tl_authexcls; red_tl_lifetime; red_tl_ghost_excl_ura.
+
+  Import TreiberClient.
+
+  (** Invariants. *)
+
+  (* Namespace for TreiberClient invariants. *)
+  Definition nTCli : namespace := (nroot .@"TCli").
+  Definition nTpush : namespace := (nroot .@"Tpush").
+  Definition nTMod : namespace := (nroot .@"TMod").
+
+  Definition push_then_pop n γs γpop : sProp n :=
+    (○ γs [(1 : SCMem.val)] ∨ GEx γpop tt)%S.
+
+  Definition push_then_pop_inv n γs γpop : sProp n :=
+    (syn_inv n nTpush (push_then_pop n γs γpop))%S.
+
+  Definition Client2StackState n γk k γs γpop : sProp n :=
+    (◆[k,2] ∗
+    ((live γk k (1/2) ∗ ○ γs ([] : list SCMem.val)) -U-[k](0)-◇ (dead γk k ∗ push_then_pop_inv n γs γpop))
+    )%S.
+
+  Definition C2Inv n γk k γs γpop : sProp n :=
+    (syn_inv n nTCli (Client2StackState n γk k γs γpop))%S.
+
+  Global Instance C2Inv_persistent n γk k γs γpop : Persistent ⟦C2Inv n γk k γs γpop, n⟧.
+  Proof.
+    unfold Persistent. iIntros "H". unfold C2Inv. rewrite red_syn_inv.
+    iDestruct "H" as "#H". auto.
+  Qed.
+
+  (** Simulation proof. *)
+
+  Lemma TreiberClient_push_spec tid n :
+    ⊢ ⟦(∀ (γk kt k γs γpop : τ{nat, 1+n}),
+      ((syn_tgt_interp_as n sndl (fun m => s_memory_black m)) ∗
+      (⤉ IsT nTMod n 1 2 s kt γs) ∗
+      (⤉ C2Inv n γk k γs γpop) ∗
+      TID(tid) ∗
+      ◇[kt](1, 1) ∗
+      (⤉ Duty(tid) [(k, 0, dead γk (k : nat) ∗ push_then_pop_inv n γs γpop)]) ∗
+      ◇[k](3, 5) ∗ ⤉(live γk (k : nat) (1/2)) ∗
+      ⋈[k])
+      -∗
+      syn_wpsim (1+n) tid ⊤
+      (fun rs rt => (⤉(syn_term_cond n tid _ rs rt))%S)
+      false false
+      (fn2th TreiberClientSpec.module "thread_push" (tt ↑))
+      (fn2th TreiberClient.module "thread_push" (tt ↑))
+    )%S,1+n⟧.
+  Proof.
+    iIntros.
+    red_tl_all; iIntros (γk); red_tl_all; iIntros (kt); red_tl_all; iIntros (k); red_tl_all; iIntros (γs); red_tl_all; iIntros (γpop).
+
+    red_tl_all. unfold C2Inv. simpl.
+
+    iEval (rewrite red_syn_inv; rewrite red_syn_wpsim; rewrite red_syn_tgt_interp_as).
+
+    iIntros "(#Mem & #IsTreiber & #C2Inv & TID & Pck & Duty & Pc & Live & k_Act)".
+
+    unfold fn2th. simpl. unfold thread_push, TreiberClientSpec.thread_push.
+    rred2r. lred2r.
+
+    iDestruct (pc_split _ _ 1 4 with "Pc") as "[Ys PcSt]".
+    iMod (pc_drop _ 1 3 ltac:(auto) 100 with "Ys") as "Ys"; [lia|].
+    iDestruct (pc_split _ _ 1 99 with "Ys") as "[Y Ys]".
+    iApply (wpsim_yieldR with "[$Duty Y]"); [lia| |].
+    { simpl. iDestruct (pcs_cons_fold with "[Y]") as "$". iFrame. }
+
+    iIntros "Duty _". rred2r. iApply wpsim_tauR. rred2r.
+
+    iApply (Treiber_push_spec nTMod (λ v, (dead γk (k : nat)) ∗ syn_inv n nTpush (push_then_pop n γs γpop))%S with "[Duty Pck PcSt Live] [-]"); [|].
+    { red_tl_all. rewrite red_syn_tgt_interp_as. iSplit; [eauto|]. iSplitR; [iFrame "#"|]. simpl.
+      iFrame. simpl.
+      iDestruct (pcs_cons_fold with "[PcSt]") as "$".
+      { simpl. iFrame. }
+      iIntros (s_st). red_tl_all. iIntros "[TStackInv _]".
+      rewrite red_syn_fupd. red_tl_all.
+      iInv "C2Inv" as "Client2" "CloseC2Inv".
+      iEval (unfold Client2StackState; simpl; red_tl_all; simpl; rewrite red_syn_until_tpromise) in "Client2".
+      iDestruct "Client2" as "[#OBL PushProm]".
+
+      iEval (unfold until_thread_promise; red_tl_all; simpl) in "PushProm".
+
+      iDestruct "PushProm" as "[#Prm [Bf | #Af]]"; simpl.
+      - iEval (red_tl_all; simpl) in "Bf". iDestruct "Bf" as "[LiveInv TStackC]".
+        iDestruct (AuthExcls.b_w_eq with "TStackInv TStackC") as "%EQ".
+        subst s_st.
+        iMod (AuthExcls.b_w_update with "TStackInv TStackC") as "[TStackInv TStackC]".
+        iMod ((FUpd_alloc _ _ _ n (nTpush) (push_then_pop n γs γpop : sProp n)%S) with "[TStackC]") as "#Pushed"; [lia| |].
+        { unfold push_then_pop. iEval (simpl; red_tl_all; simpl). auto. }
+        iDestruct (Lifetime.pending_merge with "Live LiveInv") as "Live".
+        iEval (rewrite Qp.half_half) in "Live".
+        iMod (Lifetime.pending_shot with "Live") as "#Dead".
+        iMod ("CloseC2Inv" with "[]") as "_".
+        { iEval (unfold Client2StackState; simpl; red_tl_all; simpl).
+          iFrame "#". iEval (rewrite red_syn_until_tpromise).
+          iApply until_tpromise_make2. simpl. iSplit; auto.
+          iEval (red_tl_all; simpl). iModIntro; iSplit; auto.
+        }
+        iModIntro. iFrame "∗#".
+      - iEval (red_tl_all; simpl) in "Af". iDestruct "Af" as "[Dead TStackC]".
+        by iDestruct (Lifetime.pending_not_shot with "Live Dead") as "%False".
+    }
+    Unshelve.
+    2:{ apply ndot_ne_disjoint. ss. }
+
+    iIntros (_). red_tl_all. iIntros "[[#Dead Pushed] Duty]".
+    iEval (rewrite red_syn_inv) in "Pushed". iDestruct "Pushed" as "#Pushed".
+    iMod (duty_fulfill with "[Dead Duty k_Act]") as "Duty".
+    { iFrame. simpl. unfold push_then_pop_inv. red_tl_all. rewrite red_syn_inv. auto. }
+
+    rred2r.
+    iApply (wpsim_sync with "[$Duty]"); [lia|].
+
+    iIntros "Duty _". lred2r. rred2r. iApply wpsim_tauR. rred2r.
+    iApply wpsim_ret; [eauto|].
+    iModIntro.
+    iEval (unfold term_cond). iSplit; iFrame. iPureIntro; auto.
+  Qed.
+
+  Lemma TreiberClient_pop_spec tid n :
+    ⊢ ⟦(∀ (γk k kt γs γpop : τ{nat, 1+n}),
+      ((syn_tgt_interp_as n sndl (fun m => s_memory_black m)) ∗
+      (⤉ IsT nTMod n 1 2 s kt γs) ∗
+      (⤉ C2Inv n γk k γs γpop) ∗
+      (⤉ GEx γpop tt) ∗
+      ◇[kt](1,1) ∗
+      TID(tid) ∗
+      (⤉ Duty(tid) []))
+      -∗
+      syn_wpsim (1+n) tid ⊤
+      (fun rs rt => (⤉(syn_term_cond n tid _ rs rt))%S)
+      false false
+      (fn2th TreiberClientSpec.module "thread_pop" (tt ↑))
+      (fn2th TreiberClient.module "thread_pop" (tt ↑))
+    )%S,1+n⟧.
+  Proof.
+    iIntros.
+    red_tl_all; iIntros (γk); red_tl_all; iIntros (k);
+    red_tl_all; iIntros (kt);
+    red_tl_all; iIntros (γs); red_tl_all; iIntros (γpop).
+
+    red_tl_all. unfold C2Inv. simpl.
+
+    iEval (rewrite red_syn_inv; rewrite red_syn_wpsim; rewrite red_syn_tgt_interp_as).
+
+    iIntros "(#Mem & #IsTreiber & #C2Inv & Tok & Pck & TID & Duty)".
+
+    unfold fn2th. simpl. unfold thread_pop, TreiberClientSpec.thread_pop.
+    rred2r. lred2r.
+
+    iApply (wpsim_yieldR with "[$Duty]"); [lia|].
+    iIntros "Duty _". rred2r. iApply wpsim_tauR. rred2r.
+    iEval (rewrite unfold_iter_eq; rred2r).
+    iApply (wpsim_yieldR with "[$Duty]"); [lia|].
+    iIntros "Duty _". rred2r. iApply wpsim_tauR. rred2r.
+
+    iInv "C2Inv" as "Client2" "CloseC2Inv".
+    iEval (unfold Client2StackState; simpl; red_tl_all; simpl; rewrite red_syn_until_tpromise) in "Client2".
+
+    iDestruct "Client2" as "[#Obl PushProm]".
+    iPoseProof (until_tpromise_get_tpromise with "PushProm") as "#TProm".
+    iRevert "Tok TID Duty CloseC2Inv Pck".
+    iMod (until_tpromise_ind with "[Obl PushProm] [-]") as "Ind"; cycle 2.
+    { iApply "Ind". }
+    { iSplit; iFrame; auto. }
+    iSplit.
+    - simpl. red_tl_all. iIntros "!> IH !> [LiveInv TStackC] Tok TID Duty CloseC2Inv Pck".
+      iMod ("CloseC2Inv" with "[LiveInv TStackC]") as "_".
+      { iEval (unfold Client2StackState; simpl; red_tl_all; simpl).
+        iFrame "#". iEval (rewrite red_syn_until_tpromise).
+        unfold until_thread_promise. simpl. iSplit; auto.
+        iLeft. red_tl_all. iFrame.
+      }
+
+      iApply (Treiber_pop_spec nTMod (λ ov, if ov is Some v then ⌜v = 1⌝ else (GEx γpop tt))%S with "[Duty Pck Tok] [-]"); [|].
+      { red_tl_all. rewrite red_syn_tgt_interp_as. iSplit; [eauto|]. iSplit; [iFrame "#"|].
+        iFrame. simpl.  iSplitL; [|done].
+        iIntros (s_st). red_tl_all. iIntros "[TStackInv _]".
+        rewrite red_syn_fupd. red_tl_all.
+        iInv "C2Inv" as "Client2" "CloseC2Inv".
+        iEval (unfold Client2StackState; simpl; red_tl_all; simpl; rewrite red_syn_until_tpromise) in "Client2".
+
+        iDestruct "Client2" as "[#OBL PushProm]".
+
+        iEval (unfold until_thread_promise; red_tl_all; simpl) in "PushProm".
+        iDestruct "PushProm" as "[#Prm [Bf | #Af]]"; simpl.
+        - iEval (red_tl_all; simpl) in "Bf". iDestruct "Bf" as "[LiveInv TStackC]".
+          iDestruct (AuthExcls.b_w_eq with "TStackInv TStackC") as "%EQ".
+          subst s_st.
+          iMod ("CloseC2Inv" with "[LiveInv TStackC]") as "_".
+          { iEval (unfold Client2StackState; simpl; red_tl_all; simpl).
+            iFrame "#". iEval (rewrite red_syn_until_tpromise).
+            unfold until_thread_promise. simpl. iSplit; auto.
+            iLeft. red_tl_all. iFrame.
+          }
+          iModIntro. red_tl_all. iFrame "∗#".
+        - iEval (red_tl_all; simpl) in "Af". iDestruct "Af" as "[Dead PushedInv]".
+          unfold push_then_pop_inv. rewrite red_syn_inv.
+          iInv "PushedInv" as "TStackC" "ClosePushedInv".
+          unfold push_then_pop. simpl. red_tl_all.
+          iDestruct "TStackC" as "[TStackC| Tokt]"; last first.
+          { by iDestruct (ghost_excl_exclusive with "Tok Tokt") as "%False". }
+          iDestruct (AuthExcls.b_w_eq with "TStackInv TStackC") as "%EQ".
+          subst s_st.
+          iMod (AuthExcls.b_w_update with "TStackInv TStackC") as "[TStackInv TStackC]".
+          iMod ("ClosePushedInv" with "[$Tok]") as "_".
+          iMod ("CloseC2Inv" with "[TStackC]") as "_".
+          { iEval (unfold Client2StackState; simpl; red_tl_all; simpl).
+            iFrame "#". iEval (rewrite red_syn_until_tpromise).
+            unfold until_thread_promise. simpl. iSplit; auto.
+            iRight. red_tl_all. iFrame "#".
+          }
+          iModIntro. red_tl_all. iFrame. done.
+      }
+      iIntros (rv) "PopPost".
+      destruct rv as [v|]; simpl; red_tl_all; rred2r.
+      + iDestruct "PopPost" as "[[%EQ Duty] _]". subst v.
+        iApply (wpsim_sync with "[$Duty]"); [lia|].
+        iIntros "Duty C". lred2r. rred2r. iApply wpsim_tauR. rred2r.
+        iApply wpsim_ret; [eauto|].
+        iModIntro.
+        iEval (unfold term_cond). iSplit; iFrame. iPureIntro; auto.
+      + iDestruct "PopPost" as "[[Tok Duty] Pck]".
+        iApply wpsim_tauR. rred2r.
+        iEval (rewrite unfold_iter_eq; rred2r).
+        iApply (wpsim_yieldR with "[$Duty]"); [lia|].
+        iIntros "Duty C". lred2r. rred2r. iApply wpsim_tauR. rred2r.
+        iInv "C2Inv" as "Client2" "CloseC2Inv".
+        iEval (unfold Client2StackState; simpl; red_tl_all; simpl; rewrite red_syn_until_tpromise) in "Client2".
+
+        iDestruct "Client2" as "[_ PushProm]".
+        iMod ("IH" with "[$C $PushProm] ") as "IH".
+        iApply ("IH" with "Tok TID Duty CloseC2Inv Pck").
+    - unfold push_then_pop_inv. simpl. red_tl_all. rewrite red_syn_inv.
+      iIntros "!> #[Dead PushedInv] Tok TID Duty CloseC2Inv Pck".
+      iMod ("CloseC2Inv" with "[]") as "_".
+      { iEval (unfold Client2StackState; simpl; red_tl_all; simpl).
+        iFrame "#". iEval (rewrite red_syn_until_tpromise).
+        iApply until_tpromise_make2. simpl. iSplit; auto.
+        iEval (red_tl_all; simpl). iModIntro; iSplit; auto.
+      }
+      iApply (Treiber_pop_spec nTMod (λ ov, ⌜ ov = Some (1 : SCMem.val) ⌝)%S with "[Duty Pck Tok] [-]").
+      { red_tl_all. rewrite red_syn_tgt_interp_as. iSplit; [eauto|]. iSplitR; [iFrame "#"|].
+      iFrame. iSplitL; [|done]. iIntros (s_st). red_tl_all. iIntros "[TStackInv _]".
+      rewrite red_syn_fupd. red_tl_all.
+      iInv "C2Inv" as "Client2" "CloseC2Inv".
+      iEval (unfold Client2StackState; simpl; red_tl_all; simpl; rewrite red_syn_until_tpromise) in "Client2".
+
+      iDestruct "Client2" as "[#OBL PushProm]".
+
+      iEval (unfold until_thread_promise; red_tl_all; simpl) in "PushProm".
+      iDestruct "PushProm" as "[#Prm [Bf | _]]"; simpl.
+      - iEval (red_tl_all; simpl) in "Bf". iDestruct "Bf" as "[LiveInv TStackC]".
+        iDestruct (Lifetime.pending_not_shot with "LiveInv Dead") as "%False".
+        done.
+      - (* Note: Slight proof repetition with above failed induction case. *)
+        iInv "PushedInv" as "TStackC" "ClosePushedInv".
+        unfold push_then_pop. simpl. red_tl_all.
+        iDestruct "TStackC" as "[TStackC| Tokt]"; last first.
+        { iDestruct (ghost_excl_exclusive with "Tok Tokt") as %[]. }
+        iDestruct (AuthExcls.b_w_eq with "TStackInv TStackC") as %->.
+        iMod (AuthExcls.b_w_update with "TStackInv TStackC") as "[TStackInv TStackC]".
+        iMod ("ClosePushedInv" with "[$Tok]") as "_".
+        iMod ("CloseC2Inv" with "[TStackC]") as "_".
+        { iEval (unfold Client2StackState; simpl; red_tl_all; simpl).
+          iFrame "#". iEval (rewrite red_syn_until_tpromise).
+          unfold until_thread_promise. simpl. iSplit; auto.
+          iRight. red_tl_all. iFrame "#".
+        }
+        iModIntro. red_tl_all. iFrame. done.
+    }
+    iIntros (rv) "PopPost". red_tl_all.
+    iDestruct "PopPost" as "[[%EQ Duty] _]". subst rv. rred2r.
+    iApply (wpsim_sync with "[$Duty]"); [lia|].
+    iIntros "Duty C". lred2r. rred2r. iApply wpsim_tauR. rred2r.
+    iApply wpsim_ret; [eauto|].
+    iModIntro.
+    iEval (unfold term_cond). iSplit; iFrame. iPureIntro; auto.
+    Unshelve. all: apply ndot_ne_disjoint; ss.
+  Qed.
+
+End SPEC.
