src/example/treiber/SpecHOCAP.v
@@ -1,0 +1,657 @@
+From sflib Require Import sflib.
+From Paco Require Import paco.
+Require Import Coq.Classes.RelationClasses Lia Program.
+From iris Require Import bi.big_op.
+From Fairness Require Import pind Axioms ITreeLib Red TRed IRed2 WFLibLarge.
+From Fairness Require Import FairBeh Mod Linking.
+From Fairness Require Import treiber.Code.
+From Fairness Require Import PCM IProp IPM IPropAux.
+From Fairness Require Import IndexedInvariants OpticsInterp SimWeakest.
+From Fairness Require Import TemporalLogic SCMemSpec AuthExclsRA ghost_map ExclsRA.
+
+Record maybe_null_ptr := {
+  ptr :> SCMem.val;
+  ptr_mabye_null : ptr = SCMem.val_null \/ (∃ (p : SCMem.pointer), ptr = SCMem.val_ptr p);
+}.
+Global Instance maybe_null_ptr_eq_dec : EqDecision maybe_null_ptr.
+Proof.
+  intros [p1 Pp1] [p2 Pp2].
+  unfold Decision. destruct (decide (p1 = p2)) as [->|NEQ].
+  - left. f_equal. apply proof_irrelevance.
+  - right. intros H. apply NEQ. injection H. done.
+Qed.
+
+Definition to_mnp_null : maybe_null_ptr := {| ptr := SCMem.val_null; ptr_mabye_null := or_introl eq_refl |}.
+
+Definition to_mnp_ptr ptr
+  (IsPtr : (∃ (p : SCMem.pointer), ptr = SCMem.val_ptr p)) :=
+  {| ptr := ptr; ptr_mabye_null := or_intror IsPtr |}.
+
+Section SPEC.
+
+  Context {src_state : Type}.
+  Context {src_ident : Type}.
+  Context {Client : Mod.t}.
+  Context {gvs : list nat}.
+  Context (treiberN : namespace) `{DISJ: (↑N_state_tgt :coPset) ## (↑treiberN : coPset)}.
+  Notation tgt_state := (OMod.closed_state Client (SCMem.mod gvs)).
+  Notation tgt_ident := (OMod.closed_ident Client (SCMem.mod gvs)).
+
+  Local Instance STT : StateTypes := Build_StateTypes src_state tgt_state src_ident tgt_ident.
+
+  Context `{sub : @SRA.subG Γ Σ}.
+  Context {TLRASs : TLRAs_small STT Γ}.
+  Context {TLRAS : TLRAs STT Γ Σ}.
+
+  Context {HasMEMRA: @GRA.inG memRA Γ}.
+  Context {HasAuthExcl : @GRA.inG (AuthExcls.t (list SCMem.val)) Γ}.
+  Context {HasExcl : @GRA.inG (Excls.t unit) Γ}.
+  Context {HasGhostMap : @GRA.inG (ghost_mapURA nat maybe_null_ptr) Γ}.
+
+  Ltac red_tl_all := red_tl_every; red_tl_memra; red_tl_authexcls; red_tl_ghost_map_ura.
+
+  Definition to_val (mnp : maybe_null_ptr) : SCMem.val :=
+    ptr mnp.
+
+  Fixpoint phys_list n (l : maybe_null_ptr) (L : list SCMem.val) : sProp n := (
+    match L with
+    | [] => ⌜to_val l = SCMem.val_null⌝
+    | v::tL => ∃ (p : τ{SCMem.pointer}) (r : τ{maybe_null_ptr}), ⌜to_val l = SCMem.val_ptr p⌝ ∗ (l ↦∗□ [(to_val r); v]) ∗ (phys_list n r tL)
+    end
+  )%S.
+
+  Definition LInv (n k γs : nat) (h : maybe_null_ptr) (m : gmap nat maybe_null_ptr) : sProp n  := (
+    s_ghost_map_auth γs 1 m ∗
+    [∗ n, maybe_null_ptr map] i ↦ p ∈ m, (
+      if (decide (h=p)) then
+        emp
+      else
+        ◇[k](0,1)
+    )
+  )%S.
+
+  Definition Inv (n : nat) (s : SCMem.val) (k γs γl : nat) : sProp n := (
+    ∃ (h : τ{maybe_null_ptr}) (L : τ{list SCMem.val}) (m : τ{gmap nat maybe_null_ptr,n}),
+      s ↦ (to_val h) ∗ ● γs (L : list SCMem.val) ∗
+      phys_list n h L ∗ LInv n k γl h m
+  )%S.
+
+  Definition IsT n l a s k γs : sProp n := (
+    ∃ (γl : τ{nat,n}), ◆[k,l,a] ∗ syn_inv n treiberN (Inv n s k γs γl)
+  )%S.
+
+  Global Instance IsT_persistent n l a s k γs :
+    Persistent (⟦ IsT n l a s k γs, n⟧).
+  Proof. unfold Persistent,IsT. red_tl.
+    iIntros "[%γl H]". iExists γl. red_tl.
+    rewrite red_syn_inv.
+    iDestruct "H" as "#$".
+  Qed.
+
+  Lemma Inv_unfold n s k γs γl :
+    (⟦ Inv n s k γs γl, n ⟧) -∗
+    (∃ (h : τ{maybe_null_ptr,n}) (L : τ{list SCMem.val,n}) (m : τ{gmap nat maybe_null_ptr,n}),
+      (s ↦ (to_val h)) ∗ (● γs (L : list SCMem.val)) ∗
+      ⟦ (phys_list n h L), n⟧ ∗ ⟦ LInv n k γl h m, n⟧).
+  Proof.
+    unfold Inv. iIntros "Inv".
+    repeat (red_tl; iDestruct "Inv" as "[% Inv]").
+    red_tl_all. eauto.
+  Qed.
+
+  Lemma Inv_fold n s k γs γl h L m :
+    (s ↦ (to_val h)) -∗ (● γs (L : list SCMem.val)) -∗
+    ⟦ (phys_list n h L), n⟧ -∗ ⟦ LInv n k γl h m, n⟧
+    -∗ (⟦ Inv n s k γs γl, n ⟧).
+  Proof.
+    unfold Inv. iIntros "? ? ? ?".
+    repeat (red_tl; iExists _).
+    red_tl_all. iFrame.
+  Qed.
+
+  Lemma LInv_unfold n k γs h m :
+    (⟦ LInv n k γs h m, n ⟧) -∗
+    ghost_map_auth γs 1 m ∗
+    [∗ map] a ∈ m,
+      if decide (h = a) then
+          emp
+        else
+          ◇[k](0, 1)
+    .
+  Proof.
+    unfold LInv. red_tl_all. iIntros "[$ H]".
+    rewrite red_syn_big_sepM.
+    iApply (big_sepM_mono with "H").
+    ii. des_ifs.
+  Qed.
+
+  Lemma LInv_fold n k γl h m :
+    ghost_map_auth γl 1 m -∗
+    ([∗ map] a ∈ m,
+      if decide (h = a) then
+          emp
+        else
+          ◇[k](0, 1)
+        )
+    -∗ (⟦ LInv n k γl h m, n ⟧).
+  Proof.
+    unfold LInv. red_tl_all. iIntros "$ H".
+    rewrite red_syn_big_sepM.
+    iApply (big_sepM_mono with "H").
+    ii. des_ifs.
+  Qed.
+
+
+  Lemma phys_list_unfold n l L :
+    (⟦ phys_list n l L, n ⟧) -∗
+    match L with
+    | [] => ⌜to_val l = SCMem.val_null⌝
+    | v::tL => ∃ (p : τ{SCMem.pointer,n}) (r : τ{maybe_null_ptr,n}), ⌜to_val l = SCMem.val_ptr p⌝ ∗ (l ↦∗□ [(to_val r); v]) ∗ (⟦phys_list n r tL,n⟧)
+    end.
+  Proof.
+    iIntros "H". des_ifs. simpl.
+    red_tl_all; iDestruct "H" as "[%x H]".
+    red_tl_all; iDestruct "H" as "[%r H]".
+    red_tl_all; iDestruct "H" as "[%EQ [(l.n↦ & l.d↦ & _) Phys]]".
+    iExists _,_. iFrame. done.
+  Qed.
+
+  Lemma phys_list_fold n l L :
+    (match L with
+    | [] => ⌜to_val l = SCMem.val_null⌝
+    | v::tL => ∃ (p : τ{SCMem.pointer,n}) (r : τ{maybe_null_ptr,n}), ⌜to_val l = SCMem.val_ptr p⌝ ∗ (l ↦∗□ [(to_val r); v]) ∗ (⟦phys_list n r tL,n⟧)
+    end) -∗
+    ⟦ phys_list n l L, n ⟧.
+  Proof.
+    iIntros "H". des_ifs. simpl.
+    red_tl_all; iDestruct "H" as "[%x [%r [%EQ [(l.n↦ & l.d↦ & _) Phys]]]]".
+    red_tl_all. iExists x. red_tl_all. iExists r.
+    red_tl_all. iFrame. done.
+  Qed.
+
+  Lemma phys_list_get_head n l L :
+    ⟦ phys_list n l L, n ⟧ -∗
+    □ if (decide (to_val l = SCMem.val_null)) then
+        emp
+      else (∃ (r : τ{maybe_null_ptr,n}) (h : τ{SCMem.val,n}),
+                 (l ↦∗□ [(to_val r); h]))
+    .
+  Proof.
+    iIntros "H". iDestruct (phys_list_unfold with "H") as "H". destruct L; try done.
+    all: case_decide; try done.
+    - iDestruct "H" as %EQ. done.
+    - iDestruct "H" as (p r) "[%EQ [#H _]]".
+      red_tl_all. iExists r, v. iFrame "H".
+  Qed.
+
+  Lemma Treiber_push_spec {n} (Q : SCMem.val → sProp n) (P : sProp n) tid :
+    ∀ s k γs val l a (ds : list (nat * nat * sProp n)),
+    ⊢ [@ tid, n, ⊤ @]
+          ⧼⟦(
+            (syn_tgt_interp_as n sndl (fun m => s_memory_black m))
+            ∗ (⤉ IsT n l a s k γs)
+            ∗ (⤉ Duty(tid) ds)
+            ∗ (⤉ P)
+            ∗ (∀ (S : τ{list SCMem.val, 1+n}), (⤉ (● γs (S : list SCMem.val) ∗ P))
+                  =|1+n|={⊤ ∖ ↑treiberN}=∗ (⤉ (● γs (val::S) ∗ Q val))
+              )
+            ∗ ◇[k](1,1)
+            (* TODO: Proper ord level. *)
+            ∗ ◇{List.map fst ds}(2+l,2+a)
+            )%S, 1+n⟧⧽
+            (OMod.close_itree Client (SCMem.mod gvs) (TreiberStack.push (s,val)))
+          ⧼_, ⟦(
+            (⤉ (Q val ∗ Duty(tid) ds))
+            )%S, 1+n⟧⧽
+  .
+  Proof.
+    ii. iStartTriple. red_tl_all.
+    unfold IsT. rewrite red_syn_tgt_interp_as. red_tl. simpl.
+    iIntros "(#Mem & IsT & Duty & P & AU & Ob_ks & PCS) Post".
+    iDestruct "IsT" as (γl) "IsT".
+    red_tl. rewrite red_syn_inv. iDestruct "IsT" as "#[Ob_kb IsT]".
+
+    iMod (pcs_decr _ _ 1 (1+a) with "PCS") as "[Ys PCS]"; [lia|].
+    iMod (pcs_decr _ _ 1 a with "PCS") as "[PCS CCS]"; [lia|].
+    iMod (pcs_drop _ _ 1 ltac:(lia) 1 100 with "Ys") as "Ys"; [lia|].
+    iMod (ccs_make_fine _ _ _ _ 2 with "[$Ob_kb $CCS]") as "CCS".
+
+    iEval (unfold TreiberStack.push). rred2r.
+
+    iMod ((pcs_decr _ _ 99 1) with "Ys") as "[Ys Y]"; [lia|].
+    iApply (wpsim_yieldR with "[$Duty $Y]"); [lia|].
+    iIntros "Duty _". rred2r.
+
+    iApply (SCMem_alloc_fun_spec with "[$Mem] [-]"); [lia|set_solver|].
+    iIntros (node) "(n.n↦ & n.d↦ & _)".
+    rred2r. iApply wpsim_tauR. rred2r.
+
+    iMod ((pcs_decr _ _ 98 1) with "Ys") as "[Ys Y]"; [lia|].
+    iApply (wpsim_yieldR with "[$Y $Duty]"); [lia|].
+    iIntros "Duty _". rred2r.
+
+    iApply (SCMem_store_fun_spec with "[$Mem $n.d↦] [-]"); [lia|set_solver|].
+    iIntros (?) "n.d↦". rred2r. iApply wpsim_tauR. rred2r.
+
+    move: (SCMem.val_nat 0) => next.
+
+    iRevert "n.n↦ Post Duty Ys AU P n.d↦ Ob_ks". iRevert (next). iRevert "PCS".
+
+    iMod (ccs_ind2 with "CCS [-]") as "Ind".
+    2:{ iIntros "PCS". destruct l; last first.
+        - iMod (pcs_drop _ _ 1 ltac:(auto) 2 1 with "PCS") as "PCS"; [lia|].
+          iApply ("Ind" with "PCS").
+        - iApply ("Ind" with "PCS").
+    }
+
+    iModIntro. iExists 0. iIntros "IH !> Pcs %next n.n↦ Post Duty Ys AU P n.d↦ Ob_ks".
+    iEval (rewrite unfold_iter_eq). rred2r.
+    iMod ((pcs_decr _ _ 97 1) with "Ys") as "[Ys Y]"; [lia|].
+
+    iApply (wpsim_yieldR with "[$Y $Duty]"); [lia|].
+    iIntros "Duty _". rred2r.
+
+    iInv "IsT" as "Inv" "Close". simpl.
+    iDestruct (Inv_unfold with "Inv") as (h L m) "(s↦ & γs & Phys & LInv)".
+    iApply (SCMem_load_fun_spec with "[$Mem $s↦] [-]"); [lia|solve_ndisj|].
+    iIntros (load_v) "[%EQ s↦]". subst.
+    (* Get proof that h is live for future use. *)
+    iDestruct (phys_list_get_head with "Phys") as "#h↦□".
+
+    (* Register this thread to the current waiting list for h. *)
+    iDestruct (LInv_unfold with "LInv") as "[GMap LivC]".
+    set (i := fresh (dom m)).
+    iMod (ghost_map_insert i h with "[$GMap]") as "[GMap i↪]".
+    { apply not_elem_of_dom. apply is_fresh. }
+
+    (* Close Invs *)
+    iDestruct (LInv_fold with "GMap [LivC]") as "LInv".
+    { rewrite big_sepM_insert; last first.
+      { apply not_elem_of_dom. apply is_fresh. }
+      iFrame. iClear "h↦□". case_decide; done.
+    }
+    iDestruct (Inv_fold with "s↦ γs Phys LInv") as "Inv".
+    iMod ("Close" with "Inv") as "_". move: i => i. clear dependent L m rv. rred2r.
+
+    iApply wpsim_tauR. rred2r.
+
+    iMod ((pcs_decr _ _ 96 1) with "Ys") as "[Ys Y]"; [lia|].
+    iApply (wpsim_yieldR with "[$Y $Duty]"); [lia|].
+    iIntros "Duty _". rred2r.
+
+    iApply (SCMem_store_fun_spec with "[$Mem $n.n↦] [-]"); [lia|solve_ndisj|].
+    iIntros (?) "n.n↦". rred2r. iApply wpsim_tauR. rred2r.
+
+    iMod ((pcs_decr _ _ 95 1) with "Ys") as "[Ys Y]"; [lia|].
+    iApply (wpsim_yieldR with "[$Y $Duty]"); [lia|].
+    iIntros "Duty _". rred2r.
+
+    iMod ((pcs_decr _ _ 94 1) with "Ys") as "[Ys Y]"; [lia|].
+
+    iInv "IsT" as "Inv" "Close". simpl.
+    iDestruct (Inv_unfold with "Inv") as (h' L m) "(s↦ & γs & Phys & LInv)".
+    iDestruct (phys_list_get_head with "Phys") as "#h'↦□".
+    destruct (decide (h = h')) as [<-|NEQ].
+    { (* Equal, CAS success *)
+      iApply (SCMem_cas_loc_fun_spec_gen with "[$Mem $s↦ h↦□ h'↦□] [-]"); [lia|solve_ndisj| |].
+      { des_ifs.
+        iDestruct "h↦□" as (??) "[h↦□ _]".
+        iSplit; iExists _; iFrame "h↦□".
+      }
+      iClear "h↦□ h'↦□".
+      iIntros (b) "POST".
+      iDestruct "POST" as (u) "(%EQ & s↦ & _ & _)".
+      des_ifs. destruct EQ as [-> ->].
+      iSpecialize ("AU" $! L).
+      iEval (red_tl) in "AU".
+      iEval (rewrite red_syn_fupd) in "AU".
+      iEval (red_tl_all) in "AU".
+      rred2r. iApply wpsim_tauR. rred2r.
+
+      (* Update logical stack state. *)
+      iMod ("AU" with "[$γs $P]") as "[γs Q]".
+
+      (* Update physical stack state. *)
+      iMod (SCMem.points_to_persist with "n.n↦") as "#n.n↦".
+      iMod (SCMem.points_to_persist with "n.d↦") as "#n.d↦".
+      iAssert (⌜∃ p : τ{SCMem.pointer,n}, node = SCMem.val_ptr p⌝)%I as %IsPtr.
+      { destruct node; try done. iPureIntro. eauto. }
+      iAssert (⟦ phys_list n (to_mnp_ptr node IsPtr) (val::L), n⟧)%I with "[Phys]" as "Phys".
+      { iApply phys_list_fold. simpl. des. iExists _,_. iFrame "∗#". done. }
+
+      (* Update liveness invariant *)
+      iDestruct (LInv_unfold with "LInv") as "[GMap LivC]".
+
+      iDestruct (ghost_map_lookup with "GMap i↪") as "%Lookup_i".
+      iMod (ghost_map_delete with "GMap i↪") as "GMap".
+
+      (** Create a big_opM of ◇[k](0,1). *)
+      iMod (pc_drop _ 0 1 ltac:(auto) (size (delete i m)) with "Ob_ks") as "Ob_ks"; [lia|].
+      iAssert ([∗ map] _ ∈ delete i m, ◇[k](0,1))%I with "[Ob_ks]" as "Ob_ks".
+      { set (m' := delete i m). move: m' => m'.
+        iClear "Mem IsT n.n↦ n.d↦". clear.
+        simpl in *.
+        iInduction (m') as [|id op m NotIN] "IH" using map_ind.
+        { done. }
+        rewrite big_sepM_insert; [|done].
+        rewrite map_size_insert_None; [|done].
+        iDestruct (pc_split _ _ 1 (size m) with "Ob_ks") as "[$ Ob_ks]".
+        iApply ("IH" with "Ob_ks").
+      }
+
+      (** Add it to the invariant. *)
+      iDestruct (big_sepM_delete with "LivC") as "[_ LivC]"; [apply Lookup_i|].
+      iDestruct (LInv_fold _ _ _ (to_mnp_ptr node IsPtr) with "GMap [LivC Ob_ks]") as "LInv".
+      { iDestruct (big_sepM_sep_2 with "LivC Ob_ks") as "LivC".
+        iApply (big_sepM_mono with "LivC").
+        iIntros (i' p' Lookup_i') "[H C]". des_ifs.
+      }
+
+      iDestruct (Inv_fold with "[s↦] γs Phys LInv") as "Inv".
+      { unfold to_val. iFrame. }
+      iMod ("Close" with "Inv") as "_". rred2r.
+
+      iApply (wpsim_yieldR with "[$Y $Duty]"); [lia|].
+      iIntros "Duty _". rred2r. iApply wpsim_tauR. rred2r.
+      iApply "Post". iFrame.
+    }
+    (* Different, CAS fail *)
+    iApply (SCMem_cas_loc_fun_spec_gen with "[$Mem $s↦ h↦□ h'↦□] [-]"); [lia|solve_ndisj| |].
+    { unfold to_val. des_ifs.
+      1,3: iDestruct "h'↦□" as (??) "[h'↦□ _]".
+      2,3: iDestruct "h↦□" as (??) "[h↦□ _]".
+      all: iSplit; try done; iExists _; iFrame "#".
+    }
+    iClear "h↦□ h'↦□".
+    iIntros (b) "POST".
+    iDestruct "POST" as (u) "(%EQ & s↦ & _ & _)".
+    des_ifs. all: destruct EQ as [-> ->].
+    { exfalso. clear - e NEQ. unfold to_val in e.
+      destruct h as [h Ph],h' as [h' Ph']. simpl in *. clarify.
+      assert (Ph = Ph') as -> by apply proof_irrelevance. done.
+    }
+
+    (* Update ◇[k](0,1) to use for induction *)
+    iDestruct (LInv_unfold with "LInv") as "[GMap LivC]".
+
+    iDestruct (ghost_map_lookup with "GMap i↪") as "%Lookup_i".
+    iMod (ghost_map_delete with "GMap i↪") as "GMap".
+
+    iDestruct (big_sepM_delete with "LivC") as "[Ob_k LivC]"; [apply Lookup_i|].
+    case_decide; [done|].
+    red_tl. simpl.
+
+    iDestruct (LInv_fold with "GMap LivC") as "LInv".
+    iDestruct (Inv_fold with "s↦ γs Phys LInv") as "Inv".
+    iMod ("Close" with "Inv") as "_". rred2r.
+
+    iApply wpsim_tauR. rred2r. iApply wpsim_tauR.
+
+    (* Do Induction *)
+    iMod (pcs_drop _ _ 1 ltac:(auto) 1 98 with "[$Pcs]") as "Pcs"; [lia|].
+    iMod ("IH" with "Ob_k n.n↦ Post Duty Pcs AU P n.d↦ Ob_ks") as "IH".
+    iApply "IH".
+  Qed.
+
+  Lemma Treiber_pop_spec
+        {n} (Q : (option SCMem.val) → sProp n) (P : sProp n) tid :
+    ∀ s k γs l a (ds : list (nat * nat * sProp n)),
+    ⊢ [@ tid, n, ⊤ @]
+          ⧼⟦(
+            (syn_tgt_interp_as n sndl (fun m => s_memory_black m))
+            ∗ (⤉ IsT n l a s k γs)
+            ∗ (⤉ Duty(tid) ds)
+            ∗ (⤉ P)
+            ∗ (∀ (S : τ{list SCMem.val, 1+n}), (⤉ (● γs (S : list SCMem.val) ∗ P))
+                  =|1+n|={⊤∖↑treiberN}=∗
+                  match S with
+                  | [] => (⤉ (● γs ([] : list SCMem.val) ∗ Q None))
+                  | h::t => (⤉ (● γs t ∗ Q (Some h)))
+                  end
+              )
+            ∗ ◇[k](1,1)
+            ∗ ◇{List.map fst ds}(2+l,2+a)
+            )%S, 1+n⟧⧽
+            (OMod.close_itree Client (SCMem.mod gvs) (TreiberStack.pop s))
+          ⧼rv, ⟦(
+            (⤉ (Q rv ∗ Duty(tid) ds)) ∗
+            match rv with
+            | Some _ => emp
+            | None => ◇[k](1,1)
+            end
+            )%S, 1+n⟧⧽
+  .
+  Proof.
+    ii. iStartTriple. red_tl_all.
+    unfold IsT. rewrite red_syn_tgt_interp_as. red_tl. simpl.
+    iIntros "(#Mem & IsT & Duty & P & AU & Ob_ks & PCS) Post".
+    iDestruct "IsT" as (γl) "IsT".
+    red_tl. rewrite red_syn_inv. iDestruct "IsT" as "#[Ob_kb IsT]".
+
+    iMod (pcs_decr _ _ 1 (1+a) with "PCS") as "[Ys PCS]"; [lia|].
+    iMod (pcs_decr _ _ 1 a with "PCS") as "[PCS CCS]"; [lia|].
+    iMod (pcs_drop _ _ 1 ltac:(lia) 1 102 with "Ys") as "Ys"; [lia|].
+    iMod (ccs_make_fine _ _ _ _ 2 with "[$Ob_kb $CCS]") as "CCS".
+
+    iEval (unfold TreiberStack.pop). rred2r.
+
+    iMod ((pcs_decr _ _ 101 1) with "Ys") as "[Ys Y]"; [lia|].
+    iApply (wpsim_yieldR with "[$Duty $Y]"); [lia..|].
+    iIntros "Duty _". rred2r.
+
+    iApply wpsim_tauR. rred2r.
+
+    iRevert "Post Duty Ys AU P Ob_ks". iRevert "PCS".
+
+    iMod (ccs_ind2 with "CCS [-]") as "Ind".
+    2:{ iIntros "PCS". destruct l; last first.
+        - iMod (pcs_drop _ _ 1 ltac:(auto) 2 1 with "PCS") as "PCS"; [lia|].
+        iApply ("Ind" with "PCS").
+        - iApply ("Ind" with "PCS").
+    }
+
+    iModIntro. iExists 0. iIntros "IH !> PCS Post Duty Ys AU P Ob_ks".
+    iEval (rewrite unfold_iter_eq). rred2r.
+
+    iMod ((pcs_decr _ _ 100 1) with "Ys") as "[Ys Y]"; [lia|].
+    iApply (wpsim_yieldR with "[$Duty $Y]"); [lia..|].
+    iIntros "Duty _". rred2r.
+
+    iInv "IsT" as "Inv" "Close". simpl.
+    iDestruct (Inv_unfold with "Inv") as (h St m) "(s↦ & γs & Phys & LInv)".
+
+    iApply (SCMem_load_fun_spec with "[$Mem $s↦] [-]"); [lia|solve_ndisj|].
+    iIntros (?) "[%EQ s↦]".
+    subst. rred2r. iApply wpsim_tauR. rred2r.
+    iMod ((pcs_decr _ _ 99 1) with "Ys") as "[Ys Y]"; [lia|].
+
+    destruct (decide (to_val h = to_mnp_null)) as [EQ|NEQ].
+    { (* Head is null, so stack is empty. *)
+      destruct h as [[h|h] EQh]; ss.
+      subst. injection EQ as ->. simpl in *.
+      iEval (rewrite phys_list_unfold) in "Phys".
+      des_ifs; last first.
+      { iDestruct "Phys" as (p r) "[%EQ _]". simpl in EQ. done. }
+      iClear "Phys".
+      iSpecialize ("AU" $! []). iEval (red_tl; rewrite red_syn_fupd; red_tl_all) in "AU".
+      iMod ("AU" with "[$γs $P]") as "[γs Q]".
+      iDestruct (Inv_fold with "[s↦] γs [] LInv") as "Inv".
+      { unfold to_val. iFrame. }
+      { iApply phys_list_fold. done. }
+      iMod ("Close" with "Inv") as "_". rred2r.
+
+      iApply (wpsim_yieldR with "[$Duty $Y]"); [lia..|].
+      iIntros "Duty _". rred2r.
+
+      iApply (SCMem_compare_fun_spec with "[Mem] [-]"); [|solve_ndisj| |].
+      2:{ iApply (tgt_interp_as_equiv with "Mem"). clear.
+          iStartProof. iIntros (m). simpl. red_tl_all. iSplit.
+          - iIntros "$". iPureIntro. done.
+          - iIntros "[$ _]".
+        }
+      1: lia.
+      iIntros (?) "%EQ". destruct EQ as [EQ _]. des; last done.
+      specialize (EQ EQh) as ->. rred2r.
+
+      iApply (wpsim_tauR). rred2r.
+      iApply "Post". red_tl_all. iFrame.
+    }
+
+    iDestruct (phys_list_get_head with "Phys") as "#h↦□".
+    case_decide; [done|].
+    iDestruct "h↦□" as (r d) "[h.n↦□ [h.d↦□ _]]".
+    (* Update Linv by adding myself to the ghost map, in the same way as push *)
+
+    iDestruct (LInv_unfold with "LInv") as "[GMap LivC]".
+    set (i := fresh (dom m)).
+    iMod (ghost_map_insert i h with "[$GMap]") as "[GMap i↪]".
+    { apply not_elem_of_dom. apply is_fresh. }
+
+    iDestruct (LInv_fold with "GMap [LivC]") as "LInv".
+    { rewrite big_sepM_insert; last first.
+      { apply not_elem_of_dom. apply is_fresh. }
+      iFrame. case_decide; done.
+    }
+
+    iDestruct (Inv_fold with "s↦ γs Phys LInv") as "Inv".
+    iMod ("Close" with "Inv") as "_". move: i=>i. clear dependent St m.
+
+    iApply (wpsim_yieldR with "[$Duty $Y]"); [lia..|].
+    iIntros "Duty _". rred2r.
+
+    iApply (SCMem_compare_loc_null_fun_spec with "[$Mem $h.n↦□] [-]"); [lia|solve_ndisj|].
+    iIntros (?) "[_ %EQ]". subst. rred2r.
+
+    iApply (wpsim_tauR). rred2r.
+
+    iMod ((pcs_decr _ _ 98 1) with "Ys") as "[Ys Y]"; [lia|].
+    iApply (wpsim_yieldR with "[$Duty $Y]"); [lia..|].
+    iIntros "Duty _". rred2r.
+
+    iApply (SCMem_load_fun_spec with "[$Mem $h.n↦□] [-]"); [lia|solve_ndisj|].
+    iIntros (?) "[%EQ _]". subst. rred2r.
+
+    iApply (wpsim_tauR). rred2r.
+
+    iMod ((pcs_decr _ _ 97 1) with "Ys") as "[Ys Y]"; [lia|].
+    iApply (wpsim_yieldR with "[$Duty $Y]"); [lia..|].
+    iIntros "Duty _". rred2r.
+
+    iInv "IsT" as "Inv" "Close". simpl.
+    iDestruct (Inv_unfold with "Inv") as (h' L m) "(s↦ & γs & Phys & LInv)".
+    iDestruct (phys_list_get_head with "Phys") as "#h'↦□".
+    destruct (decide (h = h')) as [<-|NEQhh'].
+    { des_ifs. iDestruct "h'↦□" as (r' d') "[h'.n↦□ [h'.d↦□ _]]". subst.
+      iDestruct (memory_ra_points_to_agree with "h.d↦□ h'.d↦□") as %<-.
+      iDestruct (memory_ra_points_to_agree with "h.n↦□ h'.n↦□") as %<-.
+
+      iDestruct (phys_list_unfold with "Phys") as "Phys".
+      destruct L as [|v tL].
+      { iDestruct "Phys" as %EQ. done. }
+      iDestruct "Phys" as (? r_new) "[%EQ_p [[#h.n↦□' [#h.d↦□' _]] Phys]]".
+
+      iDestruct (memory_ra_points_to_agree with "h.d↦□ h.d↦□'") as %<-.
+      iDestruct (memory_ra_points_to_agree with "h.n↦□ h.n↦□'") as %->.
+      clear r. iClear "h.n↦□' h.d↦□' h'.n↦□ h'.d↦□".
+
+      (* Equal, CAS success *)
+      iApply (SCMem_cas_loc_fun_spec_gen with "[$Mem $s↦] [-]"); [lia|solve_ndisj| |].
+      { des_ifs.
+        iSplit; iExists _; iFrame "h.n↦□".
+      }
+      iIntros (b) "POST".
+
+      iDestruct "POST" as (u) "(%EQ & s↦ & _ & _)".
+      des_ifs. destruct EQ as [-> ->].
+      iSpecialize ("AU" $! (d::tL)).
+      iEval (red_tl) in "AU".
+      iEval (rewrite red_syn_fupd) in "AU".
+      iEval (red_tl_all) in "AU".
+      rred2r. iApply wpsim_tauR. rred2r.
+
+      (* Update logical & physical stack state. *)
+      iMod ("AU" with "[$γs $P]") as "[γs Q]".
+
+      (* Update liveness invariant *)
+      iDestruct (LInv_unfold with "LInv") as "[GMap LivC]".
+
+      iDestruct (ghost_map_lookup with "GMap i↪") as "%Lookup_i".
+      iMod (ghost_map_delete with "GMap i↪") as "GMap".
+
+      (** Create a big_opM of ◇[k](0,1). *)
+      iMod (pc_drop _ 0 1 ltac:(auto) (size (delete i m)) with "Ob_ks") as "Ob_ks"; [lia|].
+      iAssert ([∗ map] _ ∈ delete i m, ◇[k](0,1))%I with "[Ob_ks]" as "Ob_ks".
+      { set (m' := delete i m). move: m' => m'.
+        iClear "Mem IsT h.n↦□ h.d↦□ Ob_kb". clear.
+        simpl in *.
+        iInduction (m') as [|id op m NotIN] "IH" using map_ind.
+        { done. }
+        rewrite big_sepM_insert; [|done].
+        rewrite map_size_insert_None; [|done].
+        iDestruct (pc_split _ _ 1 (size m) with "Ob_ks") as "[$ Ob_ks]".
+        iApply ("IH" with "Ob_ks").
+      }
+
+      (** Add it to the invariant. *)
+      iDestruct (big_sepM_delete with "LivC") as "[_ LivC]"; [apply Lookup_i|].
+      iDestruct (LInv_fold _ _ _ r_new with "GMap [LivC Ob_ks]") as "LInv".
+      { iDestruct (big_sepM_sep_2 with "LivC Ob_ks") as "LivC".
+        iApply (big_sepM_mono with "LivC").
+        iIntros (i' p' Lookup_i') "[H C]". des_ifs.
+      }
+
+      iDestruct (Inv_fold with "s↦ γs Phys LInv") as "Inv".
+      iMod ("Close" with "Inv") as "_". rred2r.
+
+      iMod ((pcs_decr _ _ 96 1) with "Ys") as "[Ys Y]"; [lia|].
+      iApply (wpsim_yieldR with "[$Y $Duty]"); [lia|].
+      iIntros "Duty _". rred2r.
+
+      iApply (SCMem_load_fun_spec with "[$Mem $h.d↦□] [-]"); [lia|solve_ndisj|].
+      iIntros (?) "[%EQ _]". subst. rred2r.
+
+      iApply wpsim_tauR. rred2r.
+
+      iApply "Post". red_tl. iFrame.
+    }
+    (* Different, CAS fail *)
+    iApply (SCMem_cas_loc_fun_spec_gen with "[$Mem $s↦ h.n↦□ h'↦□] [-]"); [lia|solve_ndisj| |].
+    { unfold to_val. des_ifs.
+      2: iDestruct "h'↦□" as (??) "[h'↦□ _]".
+      all: iSplit; try done; iExists _; iFrame "#".
+    }
+    iClear "h'↦□".
+    iIntros (b) "POST". iDestruct "POST" as (u) "(%EQ & s↦ & _ & _)".
+    destruct (SCMem.val_eq_dec (to_val h') (to_val h)).
+    all: destruct EQ as [-> ->].
+    { exfalso. unfold to_val in e. apply NEQhh'.
+      destruct h,h'. simpl in *. subst. f_equal. apply proof_irrelevance.
+    }
+
+    (* Update ◇[k](0,1) to use for induction *)
+    iDestruct (LInv_unfold with "LInv") as "[GMap LivC]".
+
+    iDestruct (ghost_map_lookup with "GMap i↪") as "%Lookup_i".
+    iMod (ghost_map_delete with "GMap i↪") as "GMap".
+
+    iDestruct (big_sepM_delete with "LivC") as "[Ob_k LivC]"; [apply Lookup_i|].
+    case_decide; [done|].
+    red_tl. simpl.
+
+    iDestruct (LInv_fold with "GMap LivC") as "LInv".
+    iDestruct (Inv_fold with "s↦ γs Phys LInv") as "Inv".
+    iMod ("Close" with "Inv") as "_". rred2r.
+
+    iApply wpsim_tauR. rred2r.
+
+    iApply wpsim_tauR. rred2r.
+
+    (* Do Induction *)
+    iMod (pcs_drop _ _ 1 ltac:(auto) 1 101 with "[$PCS]") as "PCS"; [lia|].
+    iMod ("IH" with "Ob_k Post Duty PCS AU P Ob_ks") as "IH".
+    iApply "IH".
+Qed.
+
+End SPEC.
+
+Global Opaque TreiberStack.pop TreiberStack.push.
